# baseURI: https://pid.bayer.com/kos/19050/technical/
# imports: http://datashapes.org/dash
# imports: http://pid.bayer.com/kos/19014/
# imports: https://pid.bayer.com/kos/19050/shacl/

@prefix metadata:  <http://topbraid.org/metadata#> .
@prefix rdf:  <http://www.w3.org/1999/02/22-rdf-syntax-ns#> .
@prefix owl:  <http://www.w3.org/2002/07/owl#> .
@prefix teamwork:  <http://topbraid.org/teamwork#> .
@prefix sh:  <http://www.w3.org/ns/shacl#> .
@prefix xsd:  <http://www.w3.org/2001/XMLSchema#> .
@prefix rdfs:  <http://www.w3.org/2000/01/rdf-schema#> .

<https://pid.bayer.com/kos/19050/hasPidUriTemplateLifecycleStatus>
        rdfs:label   "Pid Uri Template Lifecycle Status" ;
        rdf:type     owl:ObjectProperty ;
        rdfs:domain  <https://pid.bayer.com/kos/19050#PidUriTemplate> ;
        rdfs:range   <https://pid.bayer.com/kos/19050/PidUriTemplateLifecycleStatus> .

<https://pid.bayer.com/kos/19050#PidUriTemplate>
        rdfs:label       "PidUriTemplate"@en ;
        rdf:type         owl:Class ;
        rdf:type         sh:NodeShape ;
        rdfs:subClassOf  <https://pid.bayer.com/kos/19050/PID_Concepts> ;
        rdfs:comment     "Templates for PID URIs." ;
        sh:property      <https://pid.bayer.com/kos/19050/PidUriTemplate-hasIdLength> ;
        sh:property      <https://pid.bayer.com/kos/19050/PidUriTemplate-hasBaseUrl> ;
        sh:property      <https://pid.bayer.com/kos/19050#PidUriTemplate-hasPidUriTemplateLifecycleStatus> ;
        sh:property      <https://pid.bayer.com/kos/19050/PidUriTemplate-hasPidUriTemplateSuffix> ;
        sh:property      <https://pid.bayer.com/kos/19050/PidUriTemplate-hasPidUriTemplateIdType> ;
        sh:property      <https://pid.bayer.com/kos/19050/PidUriTemplate-hasRoute> ;
        sh:property      <https://pid.bayer.com/kos/19050/PidUriTemplate-type> .

<https://pid.bayer.com/kos/19050/PidUriTemplateLifecycleStatus>
        rdfs:label       "Pid Uri Template Lifecycle Status" ;
        rdf:type         owl:Class ;
        rdfs:subClassOf  <https://pid.bayer.com/kos/19050/PID_Concepts> .

<https://pid.bayer.com/kos/19050/deprecated>
        rdf:type  <https://pid.bayer.com/kos/19050/PidUriTemplateLifecycleStatus> ;
        rdf:type  <https://pid.bayer.com/kos/19050/ConsumerGroupLifecycleStatus> .

<https://pid.bayer.com/kos/19050/ConsumerGroupLifecycleStatus>
        rdfs:label       "Consumer Group Lifecycle Status" ;
        rdf:type         owl:Class ;
        rdfs:subClassOf  <https://pid.bayer.com/kos/19050/PID_Concepts> .

<https://pid.bayer.com/kos/19050#ExtendedUriTemplate-hasOrder>
        rdf:type        sh:PropertyShape ;
        sh:pattern      "^[0-9]*$" ;
        sh:description  "The order describes the order in which the extended uris are considered in the configuration of the proxy. " ;
        sh:name         "Order" ;
        sh:path         <https://pid.bayer.com/kos/19050#hasOrder> ;
        sh:minCount     1 ;
        sh:maxCount     1 ;
        sh:nodeKind     sh:Literal ;
        sh:order        "5"^^xsd:decimal ;
        sh:group        <https://pid.bayer.com/kos/19050#StandardGroup> .

<https://pid.bayer.com/kos/19050#hasOrder>
        rdfs:label    "Order" ;
        rdf:type      owl:DatatypeProperty ;
        rdfs:domain   <https://pid.bayer.com/kos/19050#ExtendedUriTemplate> ;
        rdfs:comment  "The order describes the order in which the extended URIs are considered in the configuration of the proxy." .

<https://pid.bayer.com/kos/19050#StandardGroup>
        rdfs:label  "Standard Group" ;
        rdf:type    sh:PropertyGroup ;
        sh:order    1 ;
        <http://topbraid.org/tosh#viewGroupDescription>  "" ;
        <http://topbraid.org/tosh#editGroupDescription>  "" .

<https://pid.bayer.com/kos/19050#UseHttpScheme>
        rdfs:label    "Use Http Scheme" ;
        rdf:type      owl:DatatypeProperty ;
        rdfs:domain   <https://pid.bayer.com/kos/19050#ExtendedUriTemplate> ;
        rdfs:comment  "If the variable {encodedPidUri} is used in the replacement string, the field HTTP Scheme can be used to decide whether the variable {encodedPidUri} should contain http instead of https. If HTTP Scheme is true, http is used, otherwise https." .

<https://pid.bayer.com/kos/19050#ExtendedUriTemplate>
        rdfs:label       "ExtendedUriTemplate"@en ;
        rdf:type         owl:Class ;
        rdf:type         sh:NodeShape ;
        rdfs:subClassOf  <https://pid.bayer.com/kos/19050/PID_Concepts> ;
        rdfs:comment     "Extended URI Templates." ;
        sh:property      <https://pid.bayer.com/kos/19050#ExtendedUriTemplate-hasOrder> ;
        sh:property      <https://pid.bayer.com/kos/19050/ExtendedUriTemplate-hasTargetUriMatchRegex> ;
        sh:property      <https://pid.bayer.com/kos/19050/ExtendedUriTemplate-label> ;
        sh:property      <https://pid.bayer.com/kos/19050#ExtendedUriTemplate-UseHttpScheme> ;
        sh:property      <https://pid.bayer.com/kos/19050/ExtendedUriTemplate-hasPidUriSearchRegex> ;
        sh:property      <https://pid.bayer.com/kos/19050/ExtendedUriTemplate-hasReplacementString> ;
        sh:property      <https://pid.bayer.com/kos/19050/ExtendedUriTemplate-type> .

<https://pid.bayer.com/kos/19050/ConsumerGroup-type>
        rdf:type     sh:PropertyShape ;
        sh:name      "Entity Type" ;
        sh:path      rdf:type ;
        sh:minCount  1 ;
        sh:nodeKind  sh:IRI ;
        sh:order     70 ;
        sh:group     <https://pid.bayer.com/kos/19050/TechnicalInformation> .

<https://pid.bayer.com/kos/19050/Keyword>
        sh:property  <https://pid.bayer.com/kos/19050/Keyword-type> .

<https://pid.bayer.com/kos/19050/Keyword-type>
        rdf:type     sh:PropertyShape ;
        sh:name      "Entity Type" ;
        sh:path      rdf:type ;
        sh:minCount  1 ;
        sh:nodeKind  sh:IRI ;
        sh:order     "2"^^xsd:decimal ;
        sh:group     <https://pid.bayer.com/kos/19050/TechnicalInformation> .

<https://pid.bayer.com/kos/19050/ExtendedUriTemplate-hasTargetUriMatchRegex>
        rdf:type     sh:PropertyShape ;
        sh:name      "Target URI Match Regex" ;
        sh:path      <https://pid.bayer.com/kos/19050#hasTargetUriMatchRegex> ;
        sh:minCount  1 ;
        sh:maxCount  1 ;
        sh:nodeKind  sh:Literal ;
        sh:order     1 ;
        sh:group     <https://pid.bayer.com/kos/19050#StandardGroup> ;
        sh:datatype  xsd:string .

<https://pid.bayer.com/kos/19050#hasTargetUriMatchRegex>
        rdfs:label    "hasTargetUriMatchRegex"@en ;
        rdf:type      owl:DatatypeProperty ;
        rdfs:domain   <https://pid.bayer.com/kos/19050#ExtendedUriTemplate> ;
        rdfs:range    xsd:string ;
        rdfs:comment  "A regular expression that must match the target address of an entry (e.g. the target address of a distribution endpoint) so that this Extended URI Template is applied and a proxy entry with regular expressions is created." .

<https://pid.bayer.com/kos/19050/ExtendedUriTemplate-label>
        rdf:type     sh:PropertyShape ;
        sh:name      "Name" ;
        sh:path      rdfs:label ;
        sh:minCount  1 ;
        sh:maxCount  1 ;
        sh:nodeKind  sh:Literal ;
        sh:order     0 ;
        sh:group     <https://pid.bayer.com/kos/19050#StandardGroup> ;
        sh:datatype  xsd:string .

<https://pid.bayer.com/kos/19050/taxonomies#Number>
        rdfs:label  "Number"@en ;
        rdf:type    <https://pid.bayer.com/kos/19050#PidUriTemplateIdType> .

<https://pid.bayer.com/kos/19050#hasRoute>
        rdfs:label    "hasRoute"@en ;
        rdf:type      owl:DatatypeProperty ;
        rdfs:domain   <https://pid.bayer.com/kos/19050#PidUriTemplate> ;
        rdfs:range    xsd:string ;
        rdfs:comment  "The route of a PID URI template is a definable intermediate path, which is set between the Base URL and the ID Type." .

<https://pid.bayer.com/kos/19050#hasPidUriTemplateSuffix>
        rdfs:label    "hasPidUriTemplateSuffix"@en ;
        rdf:type      owl:ObjectProperty ;
        rdfs:domain   <https://pid.bayer.com/kos/19050#PidUriTemplate> ;
        rdfs:range    <https://pid.bayer.com/kos/19050#PidUriTemplateSuffix> ;
        rdfs:comment  "The symbol at the end of the PID URI template." .

<https://pid.bayer.com/kos/19050#PidUriTemplateSuffix>
        rdfs:label       "PidUriTemplate Suffix"@en ;
        rdf:type         owl:Class ;
        rdfs:subClassOf  <https://pid.bayer.com/kos/19050/PID_Concepts> .

<https://pid.bayer.com/kos/19050/PidUriTemplate-hasIdLength>
        rdf:type     sh:PropertyShape ;
        sh:pattern   "^[0-9]+$" ;
        sh:name      "ID Length" ;
        sh:path      <https://pid.bayer.com/kos/19050#hasIdLength> ;
        sh:minCount  1 ;
        sh:maxCount  1 ;
        sh:nodeKind  sh:Literal ;
        sh:order     3 ;
        sh:group     <https://pid.bayer.com/kos/19050#StandardGroup> ;
        sh:datatype  xsd:string .

<https://pid.bayer.com/kos/19050#hasIdLength>
        rdfs:label    "hasIdLength"@en ;
        rdf:type      owl:DatatypeProperty ;
        rdfs:domain   <https://pid.bayer.com/kos/19050#PidUriTemplate> ;
        rdfs:range    xsd:string ;
        rdfs:comment  "If the PID URI Template field ID Type is of type Number, then the ID Length defines the number of digits that occur in this number. The number of a uniquely generated PID URI has a fixed number of digits, where higher digits are filled with zeros." .

<https://pid.bayer.com/kos/19050/PidUriTemplate-hasBaseUrl>
        rdf:type     sh:PropertyShape ;
        sh:name      "Base URL" ;
        sh:path      <https://pid.bayer.com/kos/19050#hasBaseUrl> ;
        sh:minCount  1 ;
        sh:maxCount  1 ;
        sh:nodeKind  sh:Literal ;
        sh:order     0 ;
        sh:group     <https://pid.bayer.com/kos/19050#StandardGroup> ;
        sh:datatype  xsd:string .

<https://pid.bayer.com/kos/19050#hasBaseUrl>
        rdfs:label    "hasBaseUrl"@en ;
        rdf:type      owl:DatatypeProperty ;
        rdfs:domain   <https://pid.bayer.com/kos/19050#PidUriTemplate> ;
        rdfs:range    xsd:string ;
        rdfs:comment  "The base URL is the prefix of both a PID URI template and the PID URIs generated from it." .

<http://pid.bayer.com/kos/19014/NetworkedResource>
        sh:property  <http://pid.bayer.com/kos/19014/NetworkedResource-type> .

<http://pid.bayer.com/kos/19014/NetworkedResource-type>
        rdf:type     sh:PropertyShape ;
        sh:name      "Endpoint Type" ;
        sh:path      rdf:type ;
        sh:minCount  1 ;
        sh:nodeKind  sh:IRI ;
        sh:order     4 ;
        sh:group     <https://pid.bayer.com/kos/19050/TechnicalInformation> .

<https://pid.bayer.com/kos/19050/ConsumerGroup-hasPidUriTemplate>
        rdf:type     sh:PropertyShape ;
        sh:name      "Pid Uri Templates" ;
        sh:path      <https://pid.bayer.com/kos/19050#hasPidUriTemplate> ;
        sh:minCount  1 ;
        sh:maxCount  1000 ;
        sh:nodeKind  sh:IRI ;
        sh:order     50 ;
        sh:group     <https://pid.bayer.com/kos/19050#StandardGroup> .

<https://pid.bayer.com/kos/19050#hasPidUriTemplate>
        rdfs:label    "hasPidUriTemplate"@en ;
        rdf:type      owl:ObjectProperty ;
        rdfs:domain   <https://pid.bayer.com/kos/19050#ConsumerGroup> ;
        rdfs:range    <https://pid.bayer.com/kos/19050#PidUriTemplate> ;
        rdfs:comment  "Which PID URI template belongs to this consumer group." .

<https://pid.bayer.com/kos/19050#hasReplacementString>
        rdfs:label    "hasReplacementString"@en ;
        rdf:type      owl:DatatypeProperty ;
        rdfs:domain   <https://pid.bayer.com/kos/19050#ExtendedUriTemplate> ;
        rdfs:range    xsd:string ;
        rdfs:comment  "The Replacement String is the new destination address to which a request should additionally be forwarded. All characters valid for a URL can be used and added. Furthermore, the two variables {targetUri} and {encodedPidUri}, as well as the RegEx groups $1 to $x from the PID URI Search Regex are available and can be added to the Replacement String. If the regular expressions match, the {targetUri} variable matches the target URI from the distribution endpoint and {encodedPidUri} variable matches the URL-encoded PID URI." .

<https://pid.bayer.com/kos/19050/PID_Concepts>
        rdfs:subClassOf  owl:Thing .

<https://pid.bayer.com/kos/19050#PidUriTemplate-hasPidUriTemplateLifecycleStatus>
        rdf:type     sh:PropertyShape ;
        sh:name      "Lifecycle Status" ;
        sh:path      <https://pid.bayer.com/kos/19050/hasPidUriTemplateLifecycleStatus> ;
        sh:minCount  1 ;
        sh:maxCount  1 ;
        sh:nodeKind  sh:IRI ;
        sh:order     "4"^^xsd:decimal ;
        sh:group     <https://pid.bayer.com/kos/19050/TechnicalInformation> .

<https://pid.bayer.com/kos/19050/367403-type>
        rdf:type     sh:PropertyShape ;
        sh:name      "Entity Type" ;
        sh:path      rdf:type ;
        sh:minCount  1 ;
        sh:nodeKind  sh:IRI ;
        sh:order     "1"^^xsd:decimal ;
        sh:group     <https://pid.bayer.com/kos/19050/TechnicalInformation> .

<https://pid.bayer.com/kos/19050#ExtendedUriTemplate-UseHttpScheme>
        rdf:type     sh:PropertyShape ;
        sh:name      "Http Scheme" ;
        sh:path      <https://pid.bayer.com/kos/19050#UseHttpScheme> ;
        sh:minCount  1 ;
        sh:maxCount  1 ;
        sh:nodeKind  sh:Literal ;
        sh:order     "4"^^xsd:decimal ;
        sh:group     <https://pid.bayer.com/kos/19050#StandardGroup> ;
        sh:datatype  xsd:boolean .

<https://pid.bayer.com/kos/19050/ExtendedUriTemplate-hasPidUriSearchRegex>
        rdf:type     sh:PropertyShape ;
        sh:name      "PID URI Search Regex" ;
        sh:path      <https://pid.bayer.com/kos/19050#hasPidUriSearchRegex> ;
        sh:minCount  1 ;
        sh:maxCount  1 ;
        sh:nodeKind  sh:Literal ;
        sh:order     2 ;
        sh:group     <https://pid.bayer.com/kos/19050#StandardGroup> ;
        sh:datatype  xsd:string .

<https://pid.bayer.com/kos/19050/ExtendedUriTemplate-hasReplacementString>
        rdf:type     sh:PropertyShape ;
        sh:name      "Replacement String" ;
        sh:path      <https://pid.bayer.com/kos/19050#hasReplacementString> ;
        sh:minCount  1 ;
        sh:maxCount  1 ;
        sh:nodeKind  sh:Literal ;
        sh:order     3 ;
        sh:group     <https://pid.bayer.com/kos/19050#StandardGroup> ;
        sh:datatype  xsd:string .

<https://pid.bayer.com/kos/19050/ExtendedUriTemplate-type>
        rdf:type     sh:PropertyShape ;
        sh:name      "Entity Type" ;
        sh:path      rdf:type ;
        sh:minCount  1 ;
        sh:nodeKind  sh:IRI ;
        sh:order     3 ;
        sh:group     <https://pid.bayer.com/kos/19050/TechnicalInformation> .

<https://pid.bayer.com/kos/19050#ConsumerGroup-hasConsumerGroupLifecycleStatus>
        rdf:type     sh:PropertyShape ;
        sh:name      "Lifecycle Status" ;
        sh:path      <https://pid.bayer.com/kos/19050/hasConsumerGroupLifecycleStatus> ;
        sh:minCount  1 ;
        sh:maxCount  1 ;
        sh:nodeKind  sh:IRI ;
        sh:order     60 ;
        sh:group     <https://pid.bayer.com/kos/19050/TechnicalInformation> .

<https://pid.bayer.com/kos/19050/hasConsumerGroupLifecycleStatus>
        rdfs:label   "Consumer Group Lifecycle Status" ;
        rdf:type     owl:ObjectProperty ;
        rdfs:domain  <https://pid.bayer.com/kos/19050#ConsumerGroup> ;
        rdfs:range   <https://pid.bayer.com/kos/19050/ConsumerGroupLifecycleStatus> .

<https://pid.bayer.com/kos/19050/PID_Concept-hasConsumerGroup>
        rdf:type     sh:PropertyShape ;
        sh:name      "Consumer Group" ;
        sh:path      <https://pid.bayer.com/kos/19050#hasConsumerGroup> ;
        sh:minCount  1 ;
        sh:maxCount  1 ;
        sh:nodeKind  sh:IRI ;
        sh:order     3 ;
        sh:group     <https://pid.bayer.com/kos/19050/TechnicalInformation> .

<https://pid.bayer.com/kos/19050#hasConsumerGroup>
        rdfs:label    "hasConsumerGroup"@en ;
        rdf:type      owl:ObjectProperty ;
        rdfs:domain   <https://pid.bayer.com/kos/19050/PID_Concept> ;
        rdfs:range    <https://pid.bayer.com/kos/19050#ConsumerGroup> ;
        rdfs:comment  "The consumer group related to the resource." .

<https://pid.bayer.com/kos/19050#hasPidUriTemplateIdType>
        rdfs:label    "hasPidUriTemplateIdType"@en ;
        rdf:type      owl:ObjectProperty ;
        rdfs:domain   <https://pid.bayer.com/kos/19050#PidUriTemplate> ;
        rdfs:range    <https://pid.bayer.com/kos/19050#PidUriTemplateIdType> ;
        rdfs:comment  "The ID Type of a PID URI template distinguishes between uniquely generated GUIDs and incremental numbers. GUIDs consist of 32 hexadecimal characters and 4 hyphens, which are generated randomly. Numbers are incremented from 0 for each PID URI template, whereby free spaces can be reused as soon as they are released after use." .

<https://pid.bayer.com/kos/19050/ConsumerGroup-hasAdRole>
        rdf:type     sh:PropertyShape ;
        sh:name      "AD Role" ;
        sh:path      <https://pid.bayer.com/kos/19050#hasAdRole> ;
        sh:minCount  1 ;
        sh:maxCount  1 ;
        sh:nodeKind  sh:Literal ;
        sh:order     20 ;
        sh:group     <https://pid.bayer.com/kos/19050#StandardGroup> ;
        sh:datatype  xsd:string .

<https://pid.bayer.com/kos/19050#hasAdRole>
        rdfs:label    "hasAdRole"@en ;
        rdf:type      owl:DatatypeProperty ;
        rdfs:domain   <https://pid.bayer.com/kos/19050#ConsumerGroup> ;
        rdfs:range    xsd:string ;
        rdfs:comment  "The Azure Active Directory role assigned to this consumer group." .

<http://pid.bayer.com/kos/19014/Resource-hasPID>
        rdfs:range  <https://pid.bayer.com/kos/19050/Identifier> .

<https://pid.bayer.com/kos/19050#ConsumerGroup>
        rdfs:label       "ConsumerGroup"@en ;
        rdf:type         owl:Class ;
        rdf:type         sh:NodeShape ;
        rdfs:subClassOf  <https://pid.bayer.com/kos/19050/PID_Concepts> ;
        rdfs:comment     "The consumer groups." ;
        sh:property      <https://pid.bayer.com/kos/19050/ConsumerGroup-type> ;
        sh:property      <https://pid.bayer.com/kos/19050/ConsumerGroup-hasPidUriTemplate> ;
        sh:property      <https://pid.bayer.com/kos/19050#ConsumerGroup-hasConsumerGroupLifecycleStatus> ;
        sh:property      <https://pid.bayer.com/kos/19050/ConsumerGroup-hasAdRole> ;
        sh:property      <https://pid.bayer.com/kos/19050/ConsumerGroup-name> ;
        sh:property      <https://pid.bayer.com/kos/19050#ConsumerGroup-hasConsumerGroupContactPerson> ;
        sh:property      <https://pid.bayer.com/kos/19050#ConsumerGroup-hasDefaultPidUriTemplate> .

<https://pid.bayer.com/kos/19050/ConsumerGroup-name>
        rdf:type     sh:PropertyShape ;
        sh:name      "Name" ;
        sh:path      rdfs:label ;
        sh:minCount  1 ;
        sh:maxCount  1 ;
        sh:nodeKind  sh:Literal ;
        sh:order     10 ;
        sh:group     <https://pid.bayer.com/kos/19050#StandardGroup> ;
        sh:datatype  xsd:string .

<https://pid.bayer.com/kos/19050/367403>
        sh:property  <https://pid.bayer.com/kos/19050/367403-type> .

<https://pid.bayer.com/kos/19050/367403->
        sh:order  "2"^^xsd:decimal .

<http://pid.bayer.com/kos/19014/Ontology-hasBaseURI>
        rdfs:range  <https://pid.bayer.com/kos/19050/Identifier> .

<https://pid.bayer.com/kos/19050#hasPidUriSearchRegex>
        rdfs:label    "hasPidUriSearchRegex"@en ;
        rdf:type      owl:DatatypeProperty ;
        rdfs:domain   <https://pid.bayer.com/kos/19050#ExtendedUriTemplate> ;
        rdfs:range    xsd:string ;
        rdfs:comment  "A regular expression that must match the PID URI of an entry (e.g. the PID URI of an entry or a distribution endpoint) so that this Extended URI Template is applied and a proxy entry with regular expressions is created." .

<https://pid.bayer.com/kos/19050/PID_Concept-type>
        rdf:type     sh:PropertyShape ;
        sh:name      "Resource Type" ;
        sh:path      rdf:type ;
        sh:minCount  1 ;
        sh:nodeKind  sh:IRI ;
        sh:order     3 ;
        sh:group     <https://pid.bayer.com/kos/19050/TechnicalInformation> .

<https://pid.bayer.com/kos/19050/PidUriTemplate-hasPidUriTemplateSuffix>
        rdf:type     sh:PropertyShape ;
        sh:name      "Suffix" ;
        sh:path      <https://pid.bayer.com/kos/19050#hasPidUriTemplateSuffix> ;
        sh:minCount  0 ;
        sh:maxCount  1 ;
        sh:nodeKind  sh:IRI ;
        sh:order     4 ;
        sh:group     <https://pid.bayer.com/kos/19050#StandardGroup> .

<https://pid.bayer.com/kos/19050/PidUriTemplate-hasPidUriTemplateIdType>
        rdf:type     sh:PropertyShape ;
        sh:name      "ID Type" ;
        sh:path      <https://pid.bayer.com/kos/19050#hasPidUriTemplateIdType> ;
        sh:minCount  1 ;
        sh:maxCount  1 ;
        sh:nodeKind  sh:IRI ;
        sh:order     2 ;
        sh:group     <https://pid.bayer.com/kos/19050#StandardGroup> .

<https://pid.bayer.com/kos/19050/PidUriTemplate-hasRoute>
        rdf:type     sh:PropertyShape ;
        sh:pattern   "^((?!.*(#|%23).*).)*$" ;
        sh:name      "Route" ;
        sh:path      <https://pid.bayer.com/kos/19050#hasRoute> ;
        sh:minCount  0 ;
        sh:maxCount  1 ;
        sh:nodeKind  sh:Literal ;
        sh:order     1 ;
        sh:group     <https://pid.bayer.com/kos/19050#StandardGroup> ;
        sh:datatype  xsd:string ;
        sh:flags     "i" .

<https://pid.bayer.com/kos/19050/PidUriTemplate-type>
        rdf:type     sh:PropertyShape ;
        sh:name      "Entity Type" ;
        sh:path      rdf:type ;
        sh:minCount  1 ;
        sh:nodeKind  sh:IRI ;
        sh:order     3 ;
        sh:group     <https://pid.bayer.com/kos/19050/TechnicalInformation> .

<https://pid.bayer.com/kos/19050/PID_Concept>
        rdfs:subClassOf  <https://pid.bayer.com/kos/19050/PID_Concepts> ;
        sh:property      <https://pid.bayer.com/kos/19050/PID_Concept-hasConsumerGroup> ;
        sh:property      <https://pid.bayer.com/kos/19050/PID_Concept-type> .

<https://pid.bayer.com/kos/19050/taxonomies#Guid>
        rdfs:label  "GUID"@en ;
        rdf:type    <https://pid.bayer.com/kos/19050#PidUriTemplateIdType> .

<https://pid.bayer.com/kos/19050/active>
        rdf:type  <https://pid.bayer.com/kos/19050/PidUriTemplateLifecycleStatus> ;
        rdf:type  <https://pid.bayer.com/kos/19050/ConsumerGroupLifecycleStatus> .

<https://pid.bayer.com/kos/19050/taxonomies#Slash>
        rdfs:label  "/"@en ;
        rdf:type    <https://pid.bayer.com/kos/19050#PidUriTemplateSuffix> .

<https://pid.bayer.com/kos/19050/taxonomies#Empty>
        rdf:type  <https://pid.bayer.com/kos/19050#PidUriTemplateSuffix> .

<https://pid.bayer.com/kos/19050#ConsumerGroup-hasConsumerGroupContactPerson>
        rdf:type        sh:PropertyShape ;
        sh:description  "The contact person for this consumer group." ;
        sh:name         "Contact Person" ;
        sh:path         <https://pid.bayer.com/kos/19050/hasConsumerGroupContactPerson> ;
        sh:minCount     1 ;
        sh:maxCount     1 ;
        sh:nodeKind     sh:Literal ;
        sh:order        30 ;
        sh:group        <https://pid.bayer.com/kos/19050#StandardGroup> ;
        sh:class        <http://pid.bayer.com/kos/19014/Person> .

<https://pid.bayer.com/kos/19050/hasConsumerGroupContactPerson>
        rdfs:label    "Contact Person" ;
        rdf:type      owl:ObjectProperty ;
        rdfs:comment  "The contact person for this consumer group." .

<https://pid.bayer.com/kos/19050#ConsumerGroup-hasDefaultPidUriTemplate>
        rdf:type     sh:PropertyShape ;
        sh:name      "Default Pid Uri Template" ;
        sh:path      <https://pid.bayer.com/kos/19050/hasDefaultPidUriTemplate> ;
        sh:minCount  0 ;
        sh:maxCount  1 ;
        sh:nodeKind  sh:IRI ;
        sh:order     "40"^^xsd:decimal ;
        sh:group     <https://pid.bayer.com/kos/19050#StandardGroup> ;
        sh:class     <https://pid.bayer.com/kos/19050#PidUriTemplate> .

<https://pid.bayer.com/kos/19050/hasDefaultPidUriTemplate>
        rdfs:label   "Default Pid Uri Template" ;
        rdf:type     owl:ObjectProperty ;
        rdfs:domain  <https://pid.bayer.com/kos/19050#ConsumerGroup> ;
        rdfs:range   <https://pid.bayer.com/kos/19050#PidUriTemplate> .

<https://pid.bayer.com/kos/19050/technical/>
        metadata:version    "1" ;
        <http://www.bayerLF.com/schema/SCHEMA_ontology#bayerGraphURI>  "https://pid.bayer.com/kos/19050/" ;
        metadata:status     metadata:UnderDevelopmentStatus ;
        rdf:type            owl:Ontology ;
        owl:imports         <https://pid.bayer.com/kos/19050/shacl/> ;
        <http://purl.org/dc/elements/1.1/title>  "PID Application Ontology" ;
        teamwork:rootClass  owl:Thing ;
        rdfs:comment        "This is the ontology specifying technical details for the COLID application." ;
        <http://www.bayerLF.com/schema/SCHEMA_ontology#bayerGraphURI>  "https://pid.bayer.com/kos/19050/technical/" ;
        <http://topbraid.org/swa#defaultNamespace>  "http://pid.bayer.com/kos/19050/pid_technical/" ;
        owl:imports         <http://datashapes.org/dash> ;
        rdfs:label          "PID Ontology Technical Open Source - DEV" .

<urn:x-evn-master:dev__pid_ontology_technical_open_source>
        rdfs:label                 "PID Ontology Technical Open Source - DEV" ;
        metadata:status            metadata:UnderDevelopmentStatus ;
        rdf:type                   <http://teamwork.topbraidlive.org/ontologyprojects#Ontology> ;
        rdf:type                   teamwork:Vocabulary ;
        rdf:type                   owl:Ontology ;
        rdfs:comment               "This is the ontology specifying technical details for the COLID application." ;
        owl:imports                <http://datashapes.org/dash> ;
        owl:imports                <http://topbraid.org/teamworkconstraints> ;
        owl:imports                <urn:x-evn-master:dev__pid_ontology_for_colid_open_source_publication> ;
        owl:imports                <urn:x-evn-master:dev__pid_ontology_shacled_for_colid_open_source_publication> ;
        <http://topbraid.org/swa#defaultNamespace>  "http://pid.bayer.com/kos/19050/pid_technical/" ;
        <http://purl.org/dc/elements/1.1/title>  "PID Application Ontology" ;
        teamwork:externalGraphURI  <https://pid.bayer.com/kos/19050/technical/> ;
        teamwork:rootClass         owl:Thing ;
        <http://www.bayerLF.com/schema/SCHEMA_ontology#bayerGraphURI>  "https://pid.bayer.com/kos/19050/technical/" ;
        <http://www.bayerLF.com/schema/SCHEMA_ontology#bayerGraphURI>  "https://pid.bayer.com/kos/19050/" ;
        metadata:version           "1" .

<http://teamwork.topbraidlive.org/ontologyprojects#Ontology>
        rdfs:subClassOf  teamwork:Vocabulary .

teamwork:Vocabulary  rdfs:subClassOf  owl:Ontology .
